theories/typing/uniq_bor.v
@@ -1,30 +1,34 @@
 From iris.proofmode Require Import tactics.
 From lrust.lifetime Require Import borrow reborrow frac_borrow.
+From lrust.lang Require Import heap.
 From lrust.typing Require Export type.
-From lrust.typing Require Import perm type_incl typing own.
+From lrust.typing Require Import perm lft_contexts typing own.
 
 Section uniq_bor.
   Context `{iris_typeG Σ}.
 
   Program Definition uniq_bor (κ:lft) (ty:type) :=
     {| ty_size := 1;
+       (* We quantify over [P]s so that the Proper lemma
+          (wrt. subtyping) works without an update. *)
        ty_own tid vl :=
-         (∃ l:loc, ⌜vl = [ #l ]⌝ ∗ &{κ} l ↦∗: ty.(ty_own) tid)%I;
+         (∃ (l:loc) P, (⌜vl = [ #l ]⌝ ∗ □ (P ↔ l ↦∗: ty.(ty_own) tid)) ∗ &{κ} P)%I;
        ty_shr κ' tid E l :=
          (∃ l':loc, &frac{κ'}(λ q', l ↦{q'} #l') ∗
             □ ∀ q' F, ⌜E ∪ mgmtE ⊆ F⌝ → q'.[κ∪κ']
                ={F, F∖E∖↑lftN}▷=∗ ty.(ty_shr) (κ∪κ') tid E l' ∗ q'.[κ∪κ'])%I
     |}.
   Next Obligation.
-    iIntros (q ty tid vl) "H". iDestruct "H" as (l) "[% _]". by subst.
+    iIntros (q ty tid vl) "H". iDestruct "H" as (l P) "[[% _] _]". by subst.
   Qed.
   Next Obligation.
     move=> κ ty E N κ' l tid q' ??/=. iIntros "#LFT Hshr Htok".
     iMod (bor_exists with "LFT Hshr") as (vl) "Hb". set_solver.
     iMod (bor_sep with "LFT Hb") as "[Hb1 Hb2]". set_solver.
     iMod (bor_exists with "LFT Hb2") as (l') "Hb2". set_solver.
-    iMod (bor_sep with "LFT Hb2") as "[EQ Hb2]". set_solver.
-    iMod (bor_persistent with "LFT EQ Htok") as "[>% $]". set_solver. subst.
+    iMod (bor_exists with "LFT Hb2") as (P) "Hb2". set_solver.
+    iMod (bor_sep with "LFT Hb2") as "[H Hb2]". set_solver.
+    iMod (bor_persistent with "LFT H Htok") as "[[>% #HPiff] $]". set_solver. subst.
     rewrite heap_mapsto_vec_singleton.
     iMod (bor_fracture (λ q, l ↦{q} #l')%I with "LFT Hb1") as "Hbf". set_solver.
     rewrite {1}bor_unfold_idx. iDestruct "Hb2" as (i) "[#Hpb Hpbown]".
@@ -33,9 +37,10 @@ Section uniq_bor.
     iExists l'. iIntros "!>{$Hbf}!#". iIntros (q'' F) "% Htok".
     iMod (inv_open with "Hinv") as "[INV Hclose]". set_solver.
     iDestruct "INV" as "[>Hbtok|#Hshr]".
-    - iMod (bor_unnest _ _ _ (l' ↦∗: ty_own ty tid)%I with "LFT [Hbtok]") as "Hb".
+    - iMod (bor_unnest _ _ _ P with "LFT [Hbtok]") as "Hb".
       { set_solver. } { iApply bor_unfold_idx. eauto. }
       iModIntro. iNext. iMod "Hb".
+      iMod (bor_iff with "LFT [] Hb") as "Hb". set_solver. by eauto.
       iMod (ty.(ty_share) with "LFT Hb Htok") as "[#$ $]"; try done. set_solver.
       iApply "Hclose". eauto.
     - iMod ("Hclose" with "[]") as "_". by eauto.
@@ -57,6 +62,41 @@ Section uniq_bor.
       by iApply (ty_shr_mono with "LFT Hκ0").
   Qed.
 
+  Global Instance subtype_uniq_mono E L :
+    Proper (flip (incl E L) ==> eqtype E L ==> subtype E L) uniq_bor.
+  Proof.
+    intros κ1 κ2 Hκ ty1 ty2 [Hty1 Hty2]. split.
+    - done.
+    - iIntros (qE qL) "#LFT HE HL *". iDestruct (Hκ with "HE HL") as "#Hκ".
+      iDestruct (subtype_own _ _ _ _ Hty1 with "LFT HE HL") as "#Hty1".
+      iDestruct (subtype_own _ _ _ _ Hty2 with "LFT HE HL") as "#Hty2".
+      iIntros "{HE HL} !# * H". iDestruct "H" as (l P) "[[% #HPiff] Hown]". subst.
+      iExists _, _. iSplitR; last by iApply (bor_shorten with "Hκ"). iSplit. done.
+      iIntros "!#". iSplit; iIntros "H".
+      + iDestruct ("HPiff" with "H") as (vl) "[??]". iExists vl. iFrame.
+        by iApply "Hty1".
+      + iDestruct "H" as (vl) "[??]". iApply "HPiff". iExists vl. iFrame.
+        by iApply "Hty2".
+    - iIntros (qE qL) "#LFT HE HL *". iDestruct (Hκ with "HE HL") as "#Hκ".
+      iDestruct (subtype_shr _ _ _ _ Hty1 with "LFT HE HL") as "#Hty".
+      iIntros "{HE HL} !# * H". iAssert (κ2 ∪ κ ⊑ κ1 ∪ κ)%I as "#Hincl'".
+      { iApply (lft_incl_glb with "[] []").
+        - iApply (lft_incl_trans with "[] Hκ"). iApply lft_le_incl.
+            apply gmultiset_union_subseteq_l.
+        - iApply lft_le_incl. apply gmultiset_union_subseteq_r. }
+      iDestruct "H" as (l') "[Hbor #Hupd]". iExists l'. iIntros "{$Hbor}!#".
+      iIntros (q' F') "% Htok".
+      iMod (lft_incl_acc with "Hincl' Htok") as (q'') "[Htok Hclose]". set_solver.
+      iMod ("Hupd" with "* [%] Htok") as "Hupd'"; try done. iModIntro. iNext.
+      iMod "Hupd'" as "[H Htok]". iMod ("Hclose" with "Htok") as "$".
+      iApply (ty_shr_mono with "LFT Hincl'"); last by iApply "Hty". done.
+  Qed.
+  Global Instance subtype_uniq_mono' E L :
+    Proper (incl E L ==> eqtype E L ==> flip (subtype E L)) uniq_bor.
+  Proof. intros ??????. apply subtype_uniq_mono. done. by symmetry. Qed.
+  Global Instance subtype_uniq_proper E L κ :
+    Proper (eqtype E L ==> eqtype E L) (uniq_bor κ).
+  Proof. split; by apply subtype_uniq_mono. Qed.
 End uniq_bor.
 
 Notation "&uniq{ κ } ty" := (uniq_bor κ ty)
@@ -73,8 +113,8 @@ Section typing.
       try by (iDestruct "Hown" as "[]" || iDestruct "Hown" as (l) "[% _]").
     iDestruct "Hown" as (l') "[EQ [Hown Hf]]". iDestruct "EQ" as %[=]. subst l'.
     iApply (fupd_mask_mono (↑lftN)). done.
-    iMod (bor_create with "LFT Hown") as "[Hbor Hext]". done.
-    iSplitL "Hbor". by simpl; eauto.
+    iMod (bor_create with "LFT Hown") as "[Hbor Hext]". done. iSplitL "Hbor".
+    { iExists _, _. erewrite <-uPred.iff_refl. auto. }
     iIntros "!>#H†". iExists _. iMod ("Hext" with "H†") as "$". by iFrame.
   Qed.
 
@@ -83,31 +123,15 @@ Section typing.
   Proof.
     iIntros (tid) "#LFT #Hord H". unfold has_type.
     destruct (eval_expr ν) as [[[|l|]|]|];
-      try by (iDestruct "H" as "[]" || iDestruct "H" as (l) "[% _]").
-    iDestruct "H" as (l') "[EQ H]". iDestruct "EQ" as %[=]. subst l'.
+      try by (iDestruct "H" as "[]" || iDestruct "H" as (l P) "[[% _] _]").
+    iDestruct "H" as (l' P) "[[EQ #HPiff] H]". iDestruct "EQ" as %[=]. subst l'.
     iApply (fupd_mask_mono (↑lftN)). done.
+    iMod (bor_iff with "LFT [] H") as "H". done. by eauto.
     iMod (rebor with "LFT Hord H") as "[H Hextr]". done.
-    iModIntro. iSplitL "H". iExists _. by eauto.
-    iIntros "H†". iExists _. by iMod ("Hextr" with "H†") as "$".
-  Qed.
-
-  Lemma lft_incl_ty_incl_uniq_bor ty κ1 κ2 :
-    ty_incl (κ1 ⊑ κ2) (&uniq{κ2}ty) (&uniq{κ1}ty).
-  Proof.
-    iIntros (tid) "#LFT #Hincl!>". iSplit; iIntros "!#*H".
-    - iDestruct "H" as (l) "[% Hown]". subst. iExists _. iSplit. done.
-      by iApply (bor_shorten with "Hincl").
-    - iAssert (κ1 ∪ κ ⊑ κ2 ∪ κ)%I as "#Hincl'".
-      { iApply (lft_incl_glb with "[] []").
-        - iApply (lft_incl_trans with "[] Hincl"). iApply lft_le_incl.
-            apply gmultiset_union_subseteq_l.
-        - iApply lft_le_incl. apply gmultiset_union_subseteq_r. }
-      iSplitL; last done. iDestruct "H" as (l') "[Hbor #Hupd]". iExists l'.
-      iFrame. iIntros "!#". iIntros (q' F) "% Htok".
-      iMod (lft_incl_acc with "Hincl' Htok") as (q'') "[Htok Hclose]". set_solver.
-      iMod ("Hupd" with "* [%] Htok") as "Hupd'"; try done. iModIntro. iNext.
-      iMod "Hupd'" as "[H Htok]". iMod ("Hclose" with "Htok") as "$".
-      by iApply (ty_shr_mono with "LFT Hincl' H").
+    iModIntro. iSplitL "H".
+    - iExists _, _. erewrite <-uPred.iff_refl. auto.
+    - iIntros "H†". iExists _, _. iMod ("Hextr" with "H†") as "$".
+      iSplitR. done. iIntros "!>!#". apply uPred.iff_refl.
   Qed.
 
   Lemma consumes_copy_uniq_bor `(!Copy ty) κ κ' q:
@@ -116,7 +140,9 @@ Section typing.
   Proof.
     iIntros (ν tid Φ E ?) "#LFT (H◁ & #H⊑ & Htok) Htl HΦ".
     iApply (has_type_wp with "H◁"). iIntros (v) "Hνv H◁". iDestruct "Hνv" as %Hνv.
-    rewrite has_type_value. iDestruct "H◁" as (l') "[Heq H↦]". iDestruct "Heq" as %[=->].
+    rewrite has_type_value. iDestruct "H◁" as (l' P) "[[Heq #HPiff] HP]".
+    iDestruct "Heq" as %[=->].
+    iMod (bor_iff with "LFT [] HP") as "H↦". set_solver. by eauto.
     iMod (lft_incl_acc with "H⊑ Htok") as (q') "[Htok Hclose]". set_solver.
     iMod (bor_acc with "LFT H↦ Htok") as "[H↦ Hclose']". set_solver.
     iDestruct "H↦" as (vl) "[>H↦ #Hown]".
@@ -124,7 +150,8 @@ Section typing.
       by rewrite ty.(ty_size_eq).
     iApply "HΦ". iFrame "∗#%". iIntros "!>!>!>H↦".
     iMod ("Hclose'" with "[H↦]") as "[H↦ Htok]". by iExists _; iFrame.
-    iMod ("Hclose" with "Htok") as "$". rewrite /has_type Hνv. iExists _. eauto.
+    iMod ("Hclose" with "Htok") as "$". rewrite /has_type Hνv.
+    iExists _, _. erewrite <-uPred.iff_refl. auto.
   Qed.
 
   Lemma typed_deref_uniq_bor_own ty ν κ κ' q q':
@@ -134,15 +161,18 @@ Section typing.
   Proof.
     iIntros (tid) "!#(#HEAP & #LFT & (H◁ & #H⊑ & Htok) & $)". wp_bind ν.
     iApply (has_type_wp with "H◁"). iIntros (v) "Hνv H◁!>". iDestruct "Hνv" as %Hνv.
-    rewrite has_type_value. iDestruct "H◁" as (l) "[Heq H↦]". iDestruct "Heq" as %[=->].
+    rewrite has_type_value. iDestruct "H◁" as (l P) "[[Heq #HPiff] HP]".
+    iDestruct "Heq" as %[=->].
+    iMod (bor_iff with "LFT [] HP") as "H↦". set_solver. by eauto.
     iMod (lft_incl_acc with "H⊑ Htok") as (q'') "[Htok Hclose]". done.
     iMod (bor_acc_cons with "LFT H↦ Htok") as "[H↦ Hclose']". done.
     iDestruct "H↦" as (vl) "[>H↦ Hown]". iDestruct "Hown" as (l') "(>% & Hown & H†)".
     subst. rewrite heap_mapsto_vec_singleton. wp_read.
     iMod ("Hclose'" with "*[H↦ Hown H†][]") as "[Hbor Htok]"; last 1 first.
     - iMod (bor_sep with "LFT Hbor") as "[_ Hbor]". done.
-      iMod (bor_sep with "LFT Hbor") as "[_ Hbor]". done.
-      iMod ("Hclose" with "Htok") as "$". iFrame "#". iExists _. eauto.
+      iMod (bor_sep _ _ _ (l' ↦∗: ty_own ty tid) with "LFT Hbor") as "[_ Hbor]". done.
+      iMod ("Hclose" with "Htok") as "$". iFrame "#". iExists _, _.
+      iFrame. iSplitR. done. by rewrite -uPred.iff_refl.
     - iFrame "H↦ H† Hown".
     - iIntros "!>(?&?&?)!>". iNext. iExists _.
       rewrite -heap_mapsto_vec_singleton. iFrame. iExists _. by iFrame.
@@ -155,19 +185,23 @@ Section typing.
   Proof.
     iIntros (tid) "!#(#HEAP & #LFT & (H◁ & #H⊑1 & Htok & #H⊑2) & $)". wp_bind ν.
     iApply (has_type_wp with "H◁"). iIntros (v) "Hνv H◁!>". iDestruct "Hνv" as %Hνv.
-    rewrite has_type_value. iDestruct "H◁" as (l) "[Heq H↦]". iDestruct "Heq" as %[=->].
+    rewrite has_type_value. iDestruct "H◁" as (l P) "[[Heq #HPiff] HP]".
+    iDestruct "Heq" as %[=->].
+    iMod (bor_iff with "LFT [] HP") as "H↦". set_solver. by eauto.
     iMod (lft_incl_acc with "H⊑1 Htok") as (q'') "[Htok Hclose]". done.
     iMod (bor_exists with "LFT H↦") as (vl) "Hbor". done.
     iMod (bor_sep with "LFT Hbor") as "[H↦ Hbor]". done.
     iMod (bor_exists with "LFT Hbor") as (l') "Hbor". done.
-    iMod (bor_sep with "LFT Hbor") as "[Heq Hbor]". done.
-    iMod (bor_persistent with "LFT Heq Htok") as "[>% Htok]". done. subst.
+    iMod (bor_exists with "LFT Hbor") as (P') "Hbor". done.
+    iMod (bor_sep with "LFT Hbor") as "[H Hbor]". done.
+    iMod (bor_persistent with "LFT H Htok") as "[[>% #HP'iff] Htok]". done. subst.
     iMod (bor_acc with "LFT H↦ Htok") as "[>H↦ Hclose']". done.
     rewrite heap_mapsto_vec_singleton.
     iApply (wp_fupd_step  _ (⊤∖↑lftN) with "[Hbor]"); try done.
       by iApply (bor_unnest with "LFT Hbor").
     wp_read. iIntros "!> Hbor". iFrame "#". iSplitL "Hbor".
-    - iExists _. iSplitR; first by auto. iApply (bor_shorten with "[] Hbor").
+    - iExists _, _. iSplitR. by auto.
+      iApply (bor_shorten with "[] Hbor").
       iApply (lft_incl_glb with "H⊑2"). iApply lft_incl_refl.
     - iApply ("Hclose" with ">"). by iMod ("Hclose'" with "[$H↦]") as "[_ $]".
   Qed.
@@ -178,12 +212,15 @@ Section typing.
   Proof.
     iIntros (ν tid Φ E ?) "#LFT (H◁ & #H⊑ & Htok) HΦ".
     iApply (has_type_wp with "H◁"). iIntros (v) "Hνv H◁". iDestruct "Hνv" as %Hνv.
-    rewrite has_type_value. iDestruct "H◁" as (l) "(Heq & H↦)". iDestruct "Heq" as %[=->].
+    rewrite has_type_value. iDestruct "H◁" as (l P) "[[Heq #HPiff] HP]".
+    iDestruct "Heq" as %[=->].
+    iMod (bor_iff with "LFT [] HP") as "H↦". set_solver. by eauto.
     iMod (lft_incl_acc with "H⊑ Htok") as (q') "[Htok Hclose]". set_solver.
     iMod (bor_acc with "LFT H↦ Htok") as "[H↦ Hclose']". set_solver.
     iDestruct "H↦" as (vl) "[>H↦ Hown]". rewrite ty.(ty_size_eq).
     iDestruct "Hown" as ">%". iApply "HΦ". iFrame "∗%#". iIntros (vl') "[H↦ Hown]".
     iMod ("Hclose'" with "[H↦ Hown]") as "[Hbor Htok]". by iExists _; iFrame.
-    iMod ("Hclose" with "Htok") as "$". rewrite /has_type Hνv. iExists _. eauto.
+    iMod ("Hclose" with "Htok") as "$". rewrite /has_type Hνv.
+    iExists _, _. erewrite <-uPred.iff_refl. auto.
   Qed.
 End typing.
