theories/lifetime/derived.v
@@ -47,6 +47,17 @@ Proof.
   iModIntro. iNext. iApply ("Hclose" with "* HP []"). by iIntros "!> $".
 Qed.
 
+Lemma bor_iff (P Q : iProp Σ) E κ :
+  ↑lftN ⊆ E →
+  lft_ctx -∗ ▷ □ (P ↔ Q) -∗ &{κ}P ={E}=∗ &{κ}Q.
+Proof.
+  iIntros (?) "#LFT #Heq Hb".
+  iMod (bor_acc_atomic_cons with "LFT Hb") as "[[HP Hclose]|[H† Hclose]]". done.
+  - iApply ("Hclose" with "[HP] []").
+      by iApply "Heq". by iIntros "!>HQ!>"; iApply "Heq".
+  - iMod "Hclose". by iApply (bor_fake with "LFT").
+Qed.
+
 Lemma bor_persistent P `{!PersistentP P} E κ q :
   ↑lftN ⊆ E →
   lft_ctx -∗ &{κ}P -∗ q.[κ] ={E}=∗ ▷ P ∗ q.[κ].
@@ -55,6 +66,7 @@ Proof.
   iMod (bor_acc with "LFT Hb Htok") as "[#HP Hob]"; first done.
   by iMod ("Hob" with "HP") as "[_ $]".
 Qed.
+
 
 Lemma lft_incl_static κ : (κ ⊑ static)%I.
 Proof.
